Tests to suport the "locals" as a special object.
Initial support for parsing locals

Locals are now resolved. Missing: locals.parameters

Consistency for local fields

Local variables AND formals

Better parsing strategy

Local parameters now resolved properly (locals``)
Better error messages

Added locals to preludeCore

Support for locals as a base ref

Correct Boogie translation of `locals`

Support for local input parameters. Now verification needs to pass.

Locals types correctly set, added missing axiom

Formals have fields for call site and for body site

Source/DafnyCore/AST/Expressions/Heap/FieldLocationExpression.cs
@@ -1,4 +1,5 @@
 ﻿using System.Collections.Generic;
+using JetBrains.Annotations;
 
 namespace Microsoft.Dafny;
 
@@ -14,10 +15,15 @@ public class FieldLocationExpression : SuffixExpr, ICloneable<FieldLocationExpre
   [FilledInDuringResolution]
   public Field ResolvedField { get; set; }
 
-  public Token Backtick { get; set; }
+  public Token Backtick { get; }
 
-  public FieldLocationExpression(Expression lhs, Token backtick, Name name) : base(name.Origin, lhs) {
+  [CanBeNull] public Token SecondBacktick { get; }
+
+  public bool DesignatesMethodInputParameter => SecondBacktick != null;
+
+  public FieldLocationExpression(Expression lhs, Token backtick, [CanBeNull] Token secondBacktick, Name name) : base(name.Origin, lhs) {
     this.Backtick = backtick;
+    this.SecondBacktick = secondBacktick;
     this.Name = name;
   }
 
@@ -28,6 +34,7 @@ public class FieldLocationExpression : SuffixExpr, ICloneable<FieldLocationExpre
       ? cloner.CloneExpr(original.ResolvedExpression) : null;
     this.Name = original.Name;
     this.Backtick = original.Backtick;
+    this.SecondBacktick = original.SecondBacktick;
   }
 
   public FieldLocationExpression Clone(Cloner cloner) {
