Source/DafnyCore/Resolver/PreType/PreTypeResolve.Expressions.cs
@@ -748,7 +748,84 @@ namespace Microsoft.Dafny {
           }
 
         case FieldLocationExpression fieldLocation: {
+            void ResolveWith(Field resolvedField, Expression resolved1) {
+              fieldLocation.ResolvedField = resolvedField;
+              ResolveExpression(resolved1, resolutionContext);
+              fieldLocation.ResolvedExpression = resolved1;
+              fieldLocation.PreType = resolved1.PreType;
+            }
+
             ResolveExpression(fieldLocation.Lhs, resolutionContext);
+            Expression resolved;
+            Field localField;
+            var name = fieldLocation.Name;
+            if (fieldLocation.Lhs is LocalsObjectExpression) {
+              if (resolutionContext.AsMethod is not { } method) {
+                ReportError(fieldLocation, "field location expressions cannot be used outside of a method");
+                fieldLocation.PreType = CreatePreTypeProxy("field-location");
+                return;
+              }
+              if (fieldLocation.DesignatesMethodInputParameter) {
+                var formal = EnclosingInputParameterFormals.Find(name.Value);
+                if (formal == null) {
+                  // Let's give an hint about declared input parameters
+                  var hints = new List<string>();
+                  hints.AddRange(EnclosingInputParameterFormals.Names
+                    .Where(n => n != null).Select(n => $"locals``{n}"));
+                  hints.AddRange(Scope.Names
+                    .Where(n => n != null).Select(n => $"locals`{n}"));
+                  ReportError(fieldLocation, "input parameter '{0}' is not declared{1}", name, DidYouMeanOneOf(hints));
+                  fieldLocation.PreType = CreatePreTypeProxy("field-location");
+                  return;
+                }
+
+                localField = formal.GetLocalFieldCallSite(method);
+                resolved = CreateObjectFieldLocation(fieldLocation.Origin, fieldLocation.Lhs, fieldLocation.Name, localField);
+                ResolveWith(localField, resolved);
+                return;
+              }
+              // We resolve the field as a local variable like for identifiers and name segments
+              var v = scope.Find(name.Value);
+              if (v == null) {
+                var f = EnclosingInputParameterFormals.Find(name.Value);
+                var hint = "";
+                if (f != null) {
+                  hint = DidYouMeanOneOf([$"locals``{name.Value}"]);
+                } else {
+                  // We only suggest variables in scope.
+                  var hints = new List<string>();
+                  hints.AddRange(Scope.Names
+                    .Where(n => n != null).Select(n => $"locals`{n}"));
+                  hints.AddRange(EnclosingInputParameterFormals.Names
+                    .Where(n => n != null).Select(n => $"locals``{n}"));
+                  hint = DidYouMeanOneOf(hints);
+                }
+                ReportError(fieldLocation, "variable '{0}' is not declared${1}", name, hint);
+                fieldLocation.PreType = CreatePreTypeProxy("field-location");
+                return;
+              }
+              if (v is not LocalVariable local) {
+                if (v is not Formal formal) {
+                  ReportError(fieldLocation, "variable '{0}' is not a local variable or a method parameter", name);
+                  fieldLocation.PreType = CreatePreTypeProxy("field-location");
+                  return;
+                }
+                localField = formal.GetLocalFieldBody(method);
+              } else {
+                localField = local.GetLocalField(method);
+              }
+              resolved = CreateObjectFieldLocation(fieldLocation.Origin, fieldLocation.Lhs, fieldLocation.Name, localField);
+              ResolveWith(localField, resolved);
+              break;
+            }
+
+            if (fieldLocation.DesignatesMethodInputParameter) {
+              // Double backtick only available if the lhs is locals, to designate input parameter memory locations.
+              // We raise an error and exit
+              ReportError(fieldLocation, "double backtick is only available with locals``name if name is a method input parameter in context");
+              fieldLocation.PreType = CreatePreTypeProxy("field-location");
+              break;
+            }
             var lhsObjType = fieldLocation.Lhs.PreType;
             lhsObjType = Constraints.FindDefinedPreType(lhsObjType, true) ?? lhsObjType;
             var innerLhsObjType = InnerTypeForBacktickLhs(lhsObjType);
@@ -776,7 +853,6 @@ namespace Microsoft.Dafny {
               return;
             }
 
-            Expression resolved;
             if (lhsObjType.IsRefType) {
               resolved = CreateObjectFieldLocation(fieldLocation.Origin, fieldLocation.Lhs, fieldLocation.Name, field);
             } else {
@@ -864,8 +940,15 @@ namespace Microsoft.Dafny {
             ResolveNestedMatchExpr(e, resolutionContext);
             break;
           }
-        case MatchExpr:
+        case MatchExpr: {
           Contract.Assert(false); // this case is always handled via NestedMatchExpr
+          break;
+        }
+        case LocalsObjectExpression locals:
+          locals.PreType = new DPreType(BuiltInTypeDecl(PreType.TypeNameObjectQ), []);
+          var objectQDecl = resolver.ProgramResolver.Program.SystemModuleManager.ObjectDecl.NonNullTypeDecl;
+          var localsType = new UserDefinedType(locals.Origin, objectQDecl.Name, objectQDecl, []);
+          locals.Type = localsType;
           break;
         default:
           Contract.Assert(false); throw new cce.UnreachableException();  // unexpected expression
@@ -875,6 +958,14 @@ namespace Microsoft.Dafny {
         // some resolution error occurred
         expr.PreType = CreatePreTypeProxy("ResolveExpression didn't compute this pre-type");
       }
+    }
+
+    private static string DidYouMeanOneOf(List<string> hints)
+    {
+      return hints.Count > 1 
+        ? " - did you mean one of " + string.Join(", ", hints.Take(hints.Count - 1)) + " or " + hints.Last()
+        : hints.Count == 1
+          ? " - did you mean " + hints.FirstOrDefault() : "";
     }
 
     private static PreType InnerTypeForBacktickLhs(PreType lhsObjType) {
@@ -895,7 +986,7 @@ namespace Microsoft.Dafny {
     // Returns also the trigger obj.fieldName
     private static DatatypeValue CreateObjectFieldLocation(IOrigin origin, Expression obj, Name fieldName, Field field) {
       return new DatatypeValue(origin, SystemModuleManager.TupleTypeName([false, false]), SystemModuleManager.TupleTypeCtorName(2),
-        [obj, new FieldLocation(fieldName, field) { Type = Type.Field }]);
+        [obj, new FieldLocation(fieldName, field) { Type = Type.Field}]);
     }
 
     private static DatatypeValue CreateObjectIndexFieldLocation(IOrigin origin, Expression obj,
@@ -2006,6 +2097,10 @@ namespace Microsoft.Dafny {
               }
               if (allowMethodCall) {
                 Contract.Assert(!e.Bindings.WasResolved); // we expect that .Bindings has not yet been processed, so we use just .ArgumentBindings in the next lines
+                var method = (MethodOrConstructor)mse.Member;
+                foreach (var inputParameter in method.Ins) {
+                  EnclosingInputParameterFormals.Push(inputParameter.Name, inputParameter);
+                }
                 foreach (var binding in e.Bindings.ArgumentBindings) {
                   ResolveExpression(binding.Actual, resolutionContext);
                 }
