Source/DafnyCore/Verifier/BoogieGenerator.cs
@@ -262,6 +262,7 @@ namespace Microsoft.Dafny {
       public readonly Bpl.Type TyTag;
       public readonly Bpl.Type TyTagFamily;
       public readonly Bpl.Expr Null;
+      public readonly Bpl.Expr Locals;
       public readonly Bpl.Constant AllocField;
       [ContractInvariantMethod]
       void ObjectInvariant() {
@@ -414,6 +415,7 @@ namespace Microsoft.Dafny {
         this.DtCtorId = new Bpl.CtorType(Token.NoToken, dtCtorId, []);
         this.AllocField = allocField;
         this.Null = new Bpl.IdentifierExpr(Token.NoToken, "null", refT);
+        this.Locals = new Bpl.IdentifierExpr(Token.NoToken, "locals", refT);
       }
     }
 
