Source/IntegrationTests/TestFiles/LitTests/LitTest/referrers/localsmemorylocation-errors.dfy
@@ -1,0 +1,15 @@
+class Test {
+  var x: int
+}
+
+method Parameters(i: Test, ghost mem_i: (object, field))
+  requires mem_i == locals`i
+{
+  var mem_i2 := locals`i;
+}
+
+method CallParameters() {
+  var t := new Test();
+  var i := new Test();
+  Parameters(t, locals`i); // Error: Precondition could not hold. Not the same local variable
+}
