Source/IntegrationTests/TestFiles/LitTests/LitTest/referrers/localsmemorylocation-resolutionerrors.dfy
@@ -1,0 +1,43 @@
+class Test {
+  var x: int
+}
+
+method LocalVars()
+  ensures locals`i == locals`i // WF Error: Local variable names cannot appear in contracts
+{
+  var i := new Test();
+  var mem_j := locals`j; // j not declared (yet)
+  var k := i``x; // Error: Double backtick only available if the lhs is locals, to designate input parameter memory locations.
+  var j := new Test();
+}
+
+
+method Parameters(i: Test, ghost mem_i: (object, field)) returns (r: Test, ghost mem_r: (object, field))
+  requires mem_i == locals`r // Error: r is not declared in ensures scope
+{
+  var mem_i2 := locals`i;
+  var mem_j := locals`j; // j not declared (yet)
+  var mem_k := locals`k; // k not declared (not at all)
+  var j := new Test();
+}
+
+method CallParameters() {
+  var test := new Test();
+  Parameters(test, locals`i); // locals`i is not defined. Did you mean in this context 'locals.``i?'
+  Parameters(test, locals``k); // locals``k is not defined. Available in context: locals``i, locals`test, locals``mem_i
+
+function FunctionParametersAreNoLocalsMemoryLocation(i: Test): int {
+  var mem_i := locals`i; // Function don't have local memory locations, all their variables are only intermediates.
+  1
+}
+
+method SingleParam(ghost mem_i: (object, field)) {
+}
+
+method CallSingleParam() {
+  SingleParam(locals``mem_j); // Did you mean locals``mem_i?
+}
+
+function NoLocals(i: Test): (object, field) {
+  locals`i // Error: field location expressions cannot be used outside of a method
+}
